Explicit Separation instance for memory to reduce term sizes.

cmap.v
@@ -97,10 +97,6 @@ Proof.
   * intros []; apply _.
 Defined.
 
-Definition cmap_erase {Ti A : Set} (m : cmap Ti A) : cmap Ti A :=
-  let (m) := m in
-  CMap (omap (λ x, '(w,β) ← maybe_Obj x; Some (Obj w β)) m).
-
 Instance cmap_sep {Ti A : Set} `{∀ τi1 τi2 : Ti, Decision (τi1 = τi2),
   Separation A} : Separation (cmap Ti A).
 Proof.
@@ -210,43 +206,3 @@ Proof.
     + by constructor; rewrite Forall_singleton.
     + inversion_clear 1; decompose_Forall_hyps; eauto using sep_unmapped_empty.
 Qed.
-
-Section cmap_erase.
-Context {Ti A : Set} `{∀ τi1 τi2 : Ti, Decision (τi1 = τi2), SeparationOps A}.
-Implicit Types m : cmap Ti A.
-Local Opaque nmap.Nempty.
-
-Lemma cmap_erase_empty : cmap_erase (∅ : cmap Ti A) = ∅.
-Proof. simpl. by rewrite omap_empty. Qed.
-Lemma dmap_erase_disjoint m1 m2 : m1 ⊥ m2 → cmap_erase m1 ⊥ cmap_erase m2.
-Proof.
-  destruct m1 as [m1], m2 as [m2]; intros Hm o; specialize (Hm o).
-  rewrite !lookup_omap. by destruct (m1 !! o) as [[]|], (m2 !! o) as [[]|].
-Qed.
-Lemma cmap_erase_union m1 m2 :
-  cmap_erase (m1 ∪ m2) = cmap_erase m1 ∪ cmap_erase m2.
-Proof.
-  sep_unfold; destruct m1 as [m1], m2 as [m2]; f_equal'; apply map_eq; intros o.
-  rewrite lookup_omap, !lookup_union_with, !lookup_omap.
-  destruct (m1 !! o) as [[]|], (m2 !! o) as [[]|]; naive_solver.
-Qed.
-Lemma dmap_erase_subseteq m1 m2 : m1 ⊆ m2 → cmap_erase m1 ⊆ cmap_erase m2.
-Proof.
-  destruct m1 as [m1], m2 as [m2]; intros Hm o; specialize (Hm o).
-  rewrite !lookup_omap. by destruct (m1 !! o) as [[]|], (m2 !! o) as [[]|].
-Qed.
-Lemma cmap_erase_difference m1 m2 :
-  m2 ⊆ m1 → cmap_erase (m1 ∖ m2) = cmap_erase m1 ∖ cmap_erase m2.
-Proof.
-  sep_unfold; destruct m1 as [m1], m2 as [m2]; intros Hm; f_equal'.
-  apply map_eq; intros o; specialize (Hm o).
-  rewrite lookup_omap, !lookup_difference_with, !lookup_omap.
-  destruct (m1 !! o) as [[]|], (m2 !! o) as [[]|];
-    simplify_option_equality; naive_solver.
-Qed.
-Lemma cmap_erase_erase m : cmap_erase (cmap_erase m) = cmap_erase m.
-Proof.
-  destruct m as [m]; f_equal'; apply map_eq; intros o.
-  rewrite !lookup_omap. by destruct (m !! o) as [[]|].
-Qed.
-End cmap_erase.
